#@base <http://dicits.ugr.es/> .
@prefix owl: <http://www.w3.org/2002/07/owl#> .
@prefix rdf: <http://www.w3.org/1999/02/22-rdf-syntax-ns#> .
@prefix xml: <http://www.w3.org/XML/1998/namespace> .
@prefix xsd: <http://www.w3.org/2001/XMLSchema#> .
@prefix rdfs: <http://www.w3.org/2000/01/rdf-schema#> .
@prefix dcterms: <http://purl.org/dc/terms/> .
@prefix foaf: <http://xmlns.com/foaf/0.1/> .
@prefix gr: <http://purl.org/goodrelations/v1#> .
@prefix skos: <http://www.w3.org/2004/02/skos/core#> .
@prefix mls: <http://www.w3.org/ns/mls> .
@prefix dmmlcc: <http://dicits.ugr.es/dmmlcc#> .
@prefix waa: <http://purl.oclc.org/NET/WebAuthentication> .
@base <http://dicits.ugr.es/dmmlcc/v1.0/> .

dmmlcc: rdf:type owl:Ontology ;
	dcterms:hasVersion 1.0 ;
	dcterms:description ""@en ;
	dcterms:title ""@en ; 
	dcterms:created "2012-09-20"^^xsd:date ;
	dcterms:issued "2014-01-14"^^xsd:date ;
	rdfs:label "Linked USDL Core"@en ;
	foaf:page <http://dicits.ugr.es/dmmlcc/start/> ;
	dcterms:creator dmmlcc:manuelparra ;
	owl:versionInfo "1.1" .

dmmlcc:manuelparra a foaf:Person;
	foaf:name "Manuel Parra";
	foaf:mbox "manuelparra@ugr.es";
	foaf:homepage <http://dicits.ugr.es/members/#manuelparra> .
	
	
#################################################################
#    Object Properties
#################################################################
dmmlcc:hasAuthentication rdf:type owl:ObjectProperty ;
	rdfs:label "hasAuthentication"@en ;
	rdfs:comment "A relation between Service and an Authentication method required by the service"@en ;
	dcterms:description "A relation beween Service and an Authentication method required by the service"@en ;
	rdfs:domain dmmlcc:Service ;
	rdfs:range dmmlcc:ServiceAuthentication ;
	.
	
	
dmmlcc:hasPart rdf:type owl:ObjectProperty ;
	rdfs:label "hasPart"@en ;
	rdfs:comment "A relation between Service and the businnes entity"@en ;
	dcterms:description "A relation between Service and the businnes entity"@en ;
	.
	
dmmlcc:hasRole rdf:type owl:ObjectProperty ;
	rdfs:label "hasRole"@en ;
	rdfs:comment "A relation between an entity and a Role tyoe"@en ;
	dcterms:description "A relation between Service and the businnes entity"@en ;
	.
	
dmmlcc:hasClassifiction rdf:type owl:ObjectProperty ;
	rdfs:label "hasClassifiction"@en ;
	rdfs:comment "A relation between the service and Catalog of the service. Link the service with de service catalog"@en ;
	dcterms:description "A relation between the service and Catalog of the service. Link the service with de service catalog"@en ;
	.
	
dmmlcc:hasSLA rdf:type owl:ObjectProperty ;
	rdfs:label "hasSLA"@en ;
	rdfs:comment "A relation between Service and SLA"@en ;
	dcterms:description "A relation between Service and SLA"@en ;
	.


dmmlcc:includes  rdf:type owl:ObjectProperty ;
	rdfs:label "includes"@en ;
	rdfs:comment "Relation of inclusion of the class Service Offering on Service"@en ;
	dcterms:description "Relation of inclusion of the class Service Offering on Service"@en ;
	rdfs:domain dmmlcc:ServiceOffering ;
	rdfs:range dmmlcc:Service ;
	.
	
dmmlcc:contains  rdf:type owl:ObjectProperty ;
	rdfs:label "contains"@en ;
	rdfs:comment "Relation with Service Input and Data"@en ;
	dcterms:description "Relation with Service Input and Data"@en ;
	rdfs:domain mls:Data ;
	rdfs:range dmmlcc:ServiceInput ;
	.
	
	
dmmlcc:hasOutputFault  rdf:type owl:ObjectProperty ;
	rdfs:label "hasOutputFault"@en ;
	rdfs:comment "Relation about Output Fault"@en ;
	dcterms:description "Relation about Output Fault"@en ;
	rdfs:subPropertyOf owl:topObjectProperty 
	.
	
dmmlcc:hasInputFault  rdf:type owl:ObjectProperty ;
	rdfs:label "hasInputFault"@en ;
	rdfs:comment "Relation about Input Fault"@en ;
	dcterms:description "Relation about Input Fault"@en ;
	rdfs:subPropertyOf owl:topObjectProperty 
	.
	
dmmlcc:hasMethod rdf:type owl:ObjectProperty ;
	rdfs:label "hasMethod"@en ;
	rdfs:comment "API Method"@en ;
	dcterms:description "API Method"@en ;
	rdfs:domain dmmlcc:Service ;
	rdfs:range dmmlcc:APIMethod ;
	.
	
dmmlcc:hasAddress rdf:type owl:ObjectProperty ;
	rdfs:label "hasAddress"@en ;
	rdfs:comment "API Service Address"@en ;
	dcterms:description "API Service Address"@en ;
	rdfs:domain dmmlcc:Service ;
	rdfs:range dmmlcc:APIMethod ;
	.


#################################################################
#    Classes
#################################################################

dmmlcc:Service rdf:Class owl:Class ;
	rdfs:subClassOf 
          [ rdf:type owl:Restriction ;
            owl:onProperty dmmlcc:hasAuthentication ;
            owl:someValuesFrom dmmlcc:ServiceAuthentication 
          ], 
          [ rdf:type owl:Restriction ;
            owl:onProperty dmmlcc:hasClassification ;
            owl:someValuesFrom dmmlcc:ServicesCatalog 
          ] , 
          [ rdf:type owl:Restriction ;
            owl:onProperty dmmlcc:hasPart ;
            owl:someValuesFrom dmmlcc:Entity 
          ]  , 
          [ rdf:type owl:Restriction ;
            owl:onProperty dmmlcc:hasOperation ;
            owl:someValuesFrom dmmlcc:Operation 
          ];
     rdfs:label "Service"@en ;
     rdfs:comment "Describing the service in a way that the information can help consumers in deciding which services are more suited for their needs."@en ;
     dcterms:description "Describing the service in a way that the information can help consumers in deciding which services are more suited for their needs."@en ;
     .


dmmlcc:ServiceAuthentication rdf:Class owl:Class ;
	rdfs:subClassOf waa:ServiceAuthentication, waa:AuthenticationMechanism ;
	rdfs:comment "ServiceAuthentication is the set of mandantory methods required to use the Service"@en ;
	dcterms:description "ServiceAuthentication is the set of mandantory methods required to use the Service"@en ;	
	.
	
	
dmmlcc:Entity rdf:type owl:Class ;
	rdfs:subClassOf
                      [ rdf:type owl:Restriction ;
                        owl:onProperty dmmlcc:hasRole ;
                        owl:someValuesFrom dmmlcc:Roles 
                      ] ;
	rdfs:subClassOf gr:BusinessEntity ;				 
	rdfs:comment "Entity that use or produce the service"@en ;
	dcterms:description "Entity that use or produce the service"@en ;	
	.


dmmlcc:Roles rdf:type owl:Class ;
	rdfs:subClassOf skos:ConceptScheme ;
	rdfs:comment "Roles taken from consumer or provider on the service"@en ;
	dcterms:description "Roles taken from consumer or provider on the service"@en ;	
	dcterms:title "List of roles availables" ;
	skos:hasTopConcept dmmlcc:Provider ;
	skos:hasTopConcept dmmlcc::Consumer ;
	.

dmmlcc:ServiceModel rdfs:Class  owl:Class ;
	rdfs:label "Service Model"@en ;
	rdfs:comment "A ServiceModel is used to represent classes of services"@en ;
	dcterms:description "A ServiceModel is used to represent classes of services"@en ;	
	rdfs:subClassOf dmmlcc:Service, gr:ProductOrService ;
	.


dmmlcc:ServiceIndividual rdfs:Class  owl:Class ;
	rdfs:label "Service Model"@en ;
	rdfs:comment "Instances of ServiceIndividual are actual services that are creating value to a network of business entities."@en ;
	dcterms:description "Instances of ServiceIndividual are actual services that are creating value to a network of business entities."@en ;	
	rdfs:subClassOf dmmlcc:Service, gr:Individual ;
	.


dmmlcc:Provider rdf:type owl:Class ;
	rdfs:subClassOf dmmlcc:Roles ;
	rdfs:comment "Entity that provides the service as a provider"@en ;
	dcterms:description "Entity that provides the service as a provider"@en ;	
	dcterms:title "Provider"@en ;
	skos:prefLabel "consumer"@en;	
	skos:broader dmmlcc:Roles ;
	.

dmmlcc:Consumer rdf:type owl:Class ;
	rdfs:subClassOf dmmlcc:Roles ;
	rdfs:comment "Entity that provides the service as a consumer"@en ;
	dcterms:description "Entity that provides the service as a consumer"@en ;	
	dcterms:title "Consumer"@en ;
	skos:prefLabel "consumer"@en;
	skos:broader dmmlcc:Roles ;
	.

dmmlcc:ServicesCatalog rdf:type owl:Class ;
	rdfs:subClassOf skos:ConceptSchema ;				 
	rdfs:comment "Services Catalog"@en ;
	dcterms:description "Services Catalog"@en ;	
	.
	
dmmlcc:SLA rdf:type owl:Class ;
	rdfs:subClassOf 
		[ rdf:type owl:Restriction ;
		  owl:onProperty dmmlcc:hasSLA ;
		  owl:someValuesFrom dmmlcc:SLA
		] ;			 
	rdfs:comment "SLA for the Service"@en ;
	dcterms:description "SLA for the Service"@en ;	
	.

dmmlcc:ServiceOffering rdf:type owl:Class ;
	rdfs:subClassOf 
		[ rdf:type owl:Restriction ;
		  owl:onProperty dmmlcc:include ;
		  owl:someValuesFrom dmmlcc:ServiceOffering
		] ;
	rdfs:label "Service Offering"@en ;
	rdfs:comment "Service Offering"@en ;
	dcterms:description "Service Offering"@en ;	
	rdfs:subClassOf gr:Offering ;
	.

dmmlcc:Operation rdf:type owl:Class ;
	rdfs:subClassOf 
		[ rdf:type owl:Restriction ;
		  owl:onProperty mls:hasOutput ;
		  owl:someValuesFrom dmmlcc:ServiceOutput
		],
		[ rdf:type owl:Restriction ;
		  owl:onProperty mls:hasInput ;
		  owl:someValuesFrom dmmlcc:ServiceInput
		], 
		[ rdf:type owl:Restriction ;
		  owl:onProperty mls:achieves ;
		  owl:someValuesFrom mls:Task
		],
		[ rdf:type owl:Restriction ;
		  owl:onProperty mls:executes ;
		  owl:someValuesFrom mls:Implementation
		], 
		[ rdf:type owl:Restriction ;
		  owl:onProperty mls:realizes ;
		  owl:someValuesFrom mls:Algorithm
		], 
		[ rdf:type owl:Restriction ;
		  owl:onProperty dmmlcc:hasInputFault ;
		  owl:someValuesFrom dmmlcc:ServiceInput
		  ], 
		[ rdf:type owl:Restriction ;
			owl:onProperty dmmlcc:hasOutputFault ;
			owl:someValuesFrom dmmlcc:ServiceOutput
		];
	rdfs:label "Execution of Service (operation)"@en ;
	rdfs:comment "Execution of Service (operation)"@en ;
	dcterms:description "Execution of a implementation"@en ;	
	.


dmmlcc:ServiceOutput rdf:type owl:Class;
	rdfs:subClassOf mls:Model, mls:ModelEvaluation, mls:DataSet ;	
	rdfs:label "Output of the operation and related service"@en ;
	rdfs:comment "Output of the operation and related service"@en ;
	dcterms:description "Output of the operation and related service"@en ;	
	.
	
dmmlcc:ServiceInput rdf:type owl:Class;
	rdfs:subClassOf mls:Data ;	
	rdfs:label "Input of the operation and related service"@en ;
	rdfs:comment "Input of the operation and related service"@en ;
	dcterms:description "Output of the operation and related service"@en ;	
	.


dmmlcc:APIMethod rdf:type owl:Class;
	rdfs:subClassOf mls:Service, rdfs:Resource, rdfs:Datatype ;	
	rdfs:label "API Method of the related service"@en ;
	rdfs:comment "API Method of the related service"@en ;
	dcterms:description "API Method of the related service"@en ;	
	.


